src/tools/parallelcomposition/derived_rulesScript.sml
@@ -64,7 +64,7 @@ REPEAT STRIP_TAC >>
 CONJUNCT2
 
                          
-  REWRITE_TAC [traceRefinement_def,traces_def,trace_def]>>
+  REWRITE_TAC [traceRefinement_def,traces_def]>>
   ASM_SIMP_TAC (std_ss++pred_setSimps.PRED_SET_ss) []>>
   REWRITE_TAC [composeMultiOperation_def]>>
   ASM_SIMP_TAC (std_ss++pred_setSimps.PRED_SET_ss) []>>
@@ -72,7 +72,7 @@ CONJUNCT2
   PAT_X_ASSUM ``?MTrn' Ded'. A`` (ASSUME_TAC o (Q.SPECL [`MTrn'`,`Ded'`])) >>
   Cases_on `MTS1 = MTS2 ∧ MTrn1 = MTrn2 ∧ Ded1 = Ded2`  >>
   ASM_SIMP_TAC (std_ss++pred_setSimps.PRED_SET_ss) []>>  
-  EVERY [REPEAT STRIP_TAC] >>
+  EVERY [REPEAT GEN_TAC] >>
   cheat
         );
 
@@ -81,8 +81,8 @@ WIP
 SET_TAC [Q.SPECL [`MTS`, `t`] trace_cases,composeMuRe_cases,composeRel_def] 
 
        
-REWRITE_TAC [composeDed_def]
-
+REWRITE_TAC [composeMuRe_def]
+REWRITE_TAC [evtrace_def]
 
  PSet_ind.SET_INDUCT_TAC 
  Induct_on `t`
@@ -91,12 +91,58 @@ PAT_X_ASSUM ``A = t`` (ASSUME_TAC o GSYM)
 FULL_SIMP_TAC (std_ss) [listTheory.EVERY_DEF]
         
 
- DISCH_TAC >> ONCE_ASM_REWRITE_TAC [] >> POP_ASSUM K_TAC
+ UNDISCH_TAC >> ONCE_ASM_REWRITE_TAC [] >> POP_ASSUM K_TAC
 
 
   SIMP_TAC (std_ss ++ SET_SPEC_ss) []
 
  REWRITE_TAC [DE_MORGAN_THM]
+
+
+
+REWRITE_TAC [traceRefinement_def]>>
+              REWRITE_TAC [traces_def]>>
+              REWRITE_TAC [trace_def]>>
+ASM_SIMP_TAC (std_ss++pred_setSimps.PRED_SET_ss) [] >>
+REPEAT GEN_TAC >>
+REPEAT EQ_TAC >>
+ASM_SIMP_TAC (std_ss++pred_setSimps.PRED_SET_ss) []>>
+
+       Cases_on `MTrn1 = MTrn2 ∧ Ded1 = Ded2`  >>
+       ASM_SIMP_TAC (std_ss++pred_setSimps.PRED_SET_ss) []>>
+       FULL_SIMP_TAC (simpLib.++(bossLib.bool_ss, boolSimps.LET_ss)) [] >>
+       REPEAT STRIP_TAC >>
+       REPEAT EQ_TAC >>
+
+
+
+        REWRITE_TAC [traceRefinement_def,traces_def]>>
+  ASM_SIMP_TAC (std_ss++pred_setSimps.PRED_SET_ss) []>>
+  REWRITE_TAC [composeMultiOperation_def]>>
+  ASM_SIMP_TAC (std_ss++pred_setSimps.PRED_SET_ss) []>>
+  REPEAT STRIP_TAC >>
+  REPEAT EQ_TAC >> REPEAT STRIP_TAC >>
+  PAT_X_ASSUM ``!t. A`` (ASSUME_TAC o (Q.SPECL [`t`]))>>
+  Q.EXISTS_TAC `Conf` >> Q.EXISTS_TAC `Conf'` >>
+  Induct_on `t` >>
+  ASM_SIMP_TAC (std_ss++pred_setSimps.PRED_SET_ss) []>>
+  REPEAT GEN_TAC >>
+
+
+REV_FULL_SIMP_TAC (std_ss) []
+  FULL_SIMP_TAC (srw_ss()) []
+REV_FULL_SIMP_TAC (arith_ss) []
+  ASM_SIMP_TAC (list_ss) []
+
+  ASM_SIMP_TAC (list_ss++pred_setSimps.PRED_SET_ss++boolSimps.LIFT_COND_ss++boolSimps.EQUIV_EXTRACT_ss) []
+Q.EXISTS_TAC `Conf` >> Q.EXISTS_TAC `Conf'` >>
+  
+ REWRITE_TAC [listTheory.LENGTH_EQ_CONS]
+        PAT_X_ASSUM ``?Conf Conf'. A`` (ASSUME_TAC o (Q.SPECL [`Conf`,`Conf'`]))
+        METIS_TAC [evtrace_def,composeMuRe_def,composeRel_def]
+        ALL_TAC
+
+        PAT_X_ASSUM ``!t. t = e::ev`` (ASSUME_TAC o (Q.SPECL [`t`,`e`,`ev`]))
 *)
 
 
@@ -105,3 +151,91 @@ FULL_SIMP_TAC (std_ss) [listTheory.EVERY_DEF]
         
 val _ = export_theory();
 
+(*
+val compose_vs_module_thm = store_thm(
+"compose_vs_module_thm", ``
+!Sym Sym' P1 P1' P2 P2' P P' S1 S1' S2 S2' S S' Conf1 Conf1' Conf2 Conf2' Conf Conf' MTrn MTrn1 MTrn2 Ded Ded1 Ded2 t1 t2 t (MTS1:('symb, 'pred1, 'state1, 'event1 + 'eventS) multransys) (MTS2:('symb, 'pred1, 'state1, 'event1 + 'eventS) multransys) (MTS: ('symb, 'pred2, 'state2, 'event2 + 'eventS) multransys).
+                 ((MTS1 ⊑ MTS2) ∧ (MTS1 = (MTrn1,Ded1)) ∧ (MTS2 = (MTrn2,Ded2)) ∧ (MTS = (MTrn,Ded)) ∧
+                 (MTrn1 Conf1 t1 Conf1') ∧ (Conf1 = (Sym,P1,S1)) ∧ (Conf1' = (Sym',P1',S1')) ∧
+                 (MTrn2 Conf2 t2 Conf2') ∧ (Conf2 = (Sym,P2,S2)) ∧ (Conf2' = (Sym',P2',S2')) ∧
+                 (MTrn Conf t Conf') ∧ (Conf = (Sym,P,S)) ∧ (Conf' = (Sym',P',S'))
+) ==> ((MTS1 || MTS) ⊑ (MTS2 || MTS)) ``
+  ,
+                 
+
+REWRITE_TAC [traceRefinement_def] >>
+ASM_SIMP_TAC (list_ss++pred_setSimps.PRED_SET_ss++boolSimps.LIFT_COND_ss++boolSimps.EQUIV_EXTRACT_ss) [] >>
+REWRITE_TAC [composeMultiOperation_def]
+REWRITE_TAC [traces_def] >>
+REWRITE_TAC [trevtrace_def]
+ASM_REWRITE_TAC [evtrace_def]
+Cases_on `MTrn1 = MTrn2` 
+ASM_SIMP_TAC (list_ss++pred_setSimps.PRED_SET_ss++boolSimps.LIFT_COND_ss++boolSimps.EQUIV_EXTRACT_ss) []
+REPEAT STRIP_TAC
+
+
+
+ASM_REWRITE_TAC [ASSUME ``Conf = (Sym,P,S)``]
+`(MTrn1 Conf [] Conf) ∨ (MTrn2 Conf' [] Conf')` by DECIDE_TAC
+              
+ASM_REWRITE_TAC[(ASSUME ``MTrn1 < MTrn2``)]
+             
+SET_TAC [Q.SPECL [`Conf`, `Conf'`] evtrace_def,composeMuRe_def,composeRel_def]        
+FULL_SIMP_TAC std_ss []            
+ASM_REWRITE_TAC [evtrace_def]
+ASM_REWRITE_TAC [composeMuRe_def]
+
+            DB.find_in "NOT" (DB.find "SUBSET");
+        DB.find "SUBSET_DEF";
+!Sym Sym' P1 P1' P2 P2' P P' S1 S1' S2 S2' S S' Conf1 Conf1' Conf2 Conf2' Conf Conf' MTrn MTrn1 MTrn2 Ded Ded1 Ded2 t1 t2 t
+
+
+
+val compose_vs_module_thm = store_thm(
+"compose_vs_module_thm", ``
+!Sym Sym' P1 P1' P2 P2' P P' S1 S1' S2 S2' S S' Conf1 Conf1' Conf2 Conf2' Conf Conf' MTrn MTrn1 MTrn2 Ded Ded1 Ded2 t1 t2 t (MTS1:('symb, 'pred1, 'state1, 'event1 + 'eventS) multransys) (MTS2:('symb, 'pred1, 'state1, 'event1 + 'eventS) multransys) (MTS: ('symb, 'pred2, 'state2, 'event2 + 'eventS) multransys).
+                 (((traces MTS1) ⊆ (traces MTS2)) ∧ (MTS1 = (MTrn1,Ded1)) ∧ (MTS2 = (MTrn2,Ded2)) ∧ (MTS = (MTrn,Ded)) ∧
+                 (MTrn1 Conf1 t1 Conf1') ∧ (Conf1 = (Sym,P1,S1)) ∧ (Conf1' = (Sym',P1',S1')) ∧
+                 (MTrn2 Conf2 t2 Conf2') ∧ (Conf2 = (Sym,P2,S2)) ∧ (Conf2' = (Sym',P2',S2')) ∧
+                 (MTrn Conf t Conf') ∧ (Conf = (Sym,P,S)) ∧ (Conf' = (Sym',P',S'))
+) ==> ((comptraces (MTS1 || MTS)) ⊆ (comptraces (MTS2 || MTS))) ``
+  ,
+       
+ASM_SIMP_TAC (list_ss++pred_setSimps.PRED_SET_ss++boolSimps.LIFT_COND_ss++boolSimps.EQUIV_EXTRACT_ss) [] >>
+REWRITE_TAC [composeMultiOperation_def]>>
+REWRITE_TAC [comptraces_def] >>
+REWRITE_TAC [traces_def] >>
+REPEAT GEN_TAC>>
+Cases_on `MTrn1 = MTrn2` >>
+ASM_SIMP_TAC (list_ss++pred_setSimps.PRED_SET_ss++boolSimps.LIFT_COND_ss++boolSimps.EQUIV_EXTRACT_ss) []>>
+ASM_REWRITE_TAC [SUBSET_DEF]>>
+ASM_SIMP_TAC (list_ss++pred_setSimps.PRED_SET_ss++boolSimps.LIFT_COND_ss++boolSimps.EQUIV_EXTRACT_ss) []>>          
+REPEAT STRIP_TAC>>
+PAT_X_ASSUM ``!x. A`` (ASSUME_TAC o (Q.SPECL [`x`]))>>
+Induct_on `x`
+
+            
+Q.EXISTS_TAC `Sym` >> Q.EXISTS_TAC `P` >>
+            Q.EXISTS_TAC `S1` >> Q.EXISTS_TAC `S2` >>
+            Q.EXISTS_TAC `Sym'` >> Q.EXISTS_TAC `P'` >>
+            Q.EXISTS_TAC `S1'` >> Q.EXISTS_TAC `S2'` >>
+      IMP_RES_TAC  composeMuRe_def
+METIS_TAC [composeMuRe_def,composeRel_def] 
+
+          Q.SPECL [`P`,`S1`,`S2`,`Sym'`,`P'`,`S1'`,`S2'`]
+
+
+
+          !Sym Sym' P1 P1' P2 P2' P P' S1 S1' S2 S2' S S' Conf1 Conf1' Conf2 Conf2' Conf Conf' MTrn MTrn1 MTrn2 Ded Ded1 Ded2 t1 t2 t (MTS1:('symb, 'pred1, 'state1, 'event1 + 'eventS) multransys) (MTS2:('symb, 'pred1, 'state1, 'event1 + 'eventS) multransys).
+                 ((MTrn1 Conf1 t1 Conf1') ∧ (Conf1 = (Sym,P1,S1)) ∧ (Conf1' = (Sym',P1',S1')) ∧
+                 (MTrn2 Conf2 t2 Conf2') ∧ (Conf2 = (Sym,P2,S2)) ∧ (Conf2' = (Sym',P2',S2'))
+) ==> (( ((MTrn1,Ded1) || (MTrn2,Ded2))) = ( ((MTrn2,Ded2) || (MTrn1,Ded1))))
+
+
+  REWRITE_TAC [composeMultiOperation_def]>>
+REWRITE_TAC [comptraces_def]>>
+ASM_SIMP_TAC (list_ss++pred_setSimps.PRED_SET_ss++boolSimps.LIFT_COND_ss++boolSimps.EQUIV_EXTRACT_ss) []>>
+REPEAT STRIP_TAC >>
+       REPEAT EQ_TAC >>
+       REPEAT STRIP_TAC >>
+*)
